\section{Embedding}

\begin{frame}
\frametitle{Outline}

\tableofcontents[currentsection]
\end{frame}


\subsection{Presentation}

\begin{frame}
\frametitle{Main idea}

\begin{block}{Main idea:}
  \begin{itemize}
  \item term embedding using HOAS (deep)
  \item translation of HOL terms into Dedukti propositions
    (deep~$\to$~shallow)
  \item proofs as rewriting rules (shallow)
  \end{itemize}
\end{block}

\end{frame}


\begin{frame}
\frametitle{HOL as a first order theory [Dowek et al. 1999]}

Simple types:
\begin{itemize}
\item $o$
\item $a \to b$
\end{itemize}

\vspace{0.5cm}

Simply-typed terms:
\begin{itemize}
\item $x$, $\lambda x.t$, $t\ u$
\item constants: $=$, logical connectives
\end{itemize}

\vspace{0.5cm}

A set of inference rules:
\begin{mathpar}
  \inferrule*{ }{\vdash t = t}

  \inferrule*{\Gamma \vdash p \Leftrightarrow q\\\Delta \vdash
    p}{\Gamma \cup \Delta \vdash q}
\end{mathpar}

\end{frame}


\begin{frame}
\frametitle{Zoom on inference rules}

Inference rules:
\begin{mathpar}
  \inferrule*{ }{\vdash t = t}

  \inferrule*{\Gamma \vdash p \Leftrightarrow q\\\Delta \vdash
    p}{\Gamma \cup \Delta \vdash q}
\end{mathpar}

\vspace{0.5cm}

Theorem $\Gamma \vdash p$:
\begin{itemize}
\item $\Gamma$: set of terms of type $o$
\item $p$: term of type $o$
\end{itemize}

\vspace{0.5cm}

\begin{itemize}
\item LCF : theorems as inhabitants of an abstract data-type
\end{itemize}

\end{frame}


\subsection{Embedding}

\begin{frame}[fragile]
\frametitle{Types and terms [SchÃ¼rmann and Stehr 2006]}

\begin{block}{Types:}
\begin{lstlisting}
htype: Type.
  o: htype.
  $\ \mapsto\ $: htype ->$\ $ htype ->$\ $ htype.
\end{lstlisting}
\end{block}

\begin{overprint}
\onslide<1>
\begin{block}{Terms:}
\begin{lstlisting}
hterm: htype -> Type.
  $\lambda$: (hterm a ->$\ $hterm b) ->$\ $hterm (a $\mapsto$ b).
  $\alpha$: hterm (a $\mapsto$ b) ->$\ $hterm a ->$\ $hterm b.
  $\dots$
\end{lstlisting}
\end{block}

\onslide<2>
\begin{block}{Terms:}
\begin{lstlisting}
hterm: htype -> Type.
  $\lambda$: (hterm a ->$\ $hterm b) ->$\ $hterm (a $\mapsto$ b).
  $\alpha$: hterm (a $\mapsto$ b) ->$\ $hterm a ->$\ $hterm b.
  $\dot{\to}$: hterm (o $\mapsto$ (o $\mapsto$ o)).
  $\dot{\forall}$: hterm ((a $\mapsto$ o) $\mapsto$ o).
  $\dot{=}$: hterm (a $\mapsto$ (a $\mapsto$ o)).
  $\dots$
\end{lstlisting}
\end{block}
\end{overprint}

\end{frame}


\begin{frame}[fragile]
\frametitle{$\beta$-reduction}

\begin{block}{$\beta$-reduction:}
\begin{lstlisting}
[a b f x] $\alpha$ ($\lambda$ f) x -->$\ $f x.
\end{lstlisting}
\end{block}

\vspace{0.5cm}

\begin{block}{Notation:}
\begin{lstlisting}
  $\alpha$ f t u $\triangleq$ $\alpha$ ($\alpha$ f t) u
\end{lstlisting}
\end{block}
\end{frame}


\begin{frame}[fragile]
\frametitle{$\varepsilon$ translation}

\lstinline!$\varepsilon$: hterm o -> Type!
\begin{itemize}
\item unary predicate symbol
\item injects a term $t$ of type $o$ into a the proposition
  $\varepsilon\ t$
\item defines a translation from the embedding into Dedukti terms
\item \alert{gives an elimination scheme to each constant}
\end{itemize}

\vspace{0.5cm}

\begin{block}{Translation:}
\begin{lstlisting}
[a b] $\varepsilon$($\alpha\ \dot{\to}$ a b) -->$\ \varepsilon$ a -> $\ \varepsilon$ b.
[a f] $\varepsilon$ ($\alpha\ \dot{\forall}$ ($\lambda$ f)) -->$\ $b: hterm a -> $\ \varepsilon$ (f b).
[a x y] $\varepsilon$ ($\alpha\ \dot{=}$ x y) -->
  P: hterm (a $\mapsto$ o) -> $\ \varepsilon$ ($\alpha$ P x) -> $\ \varepsilon$ ($\alpha$ P y).
$\dots$
\end{lstlisting}
\end{block}

\end{frame}


\begin{frame}[fragile]
\frametitle{Example of an inference rule}

\begin{mathpar}
  \inferrule*{ }{\vdash t = t}
\end{mathpar}

\begin{block}{Encoding:}
\lstinline!refl: a: htype -> t: hterm a -> $\varepsilon\ $ ($\alpha\ \dot{=}\ $t t).!

\begin{overprint}
\onslide<1>
\lstinline![a t] refl a t --> ?!
\onslide<2>
\lstinline![a t] refl a t --> P: hterm (a $\ \mapsto\ $o) =>$\ $h: $\varepsilon\ $($\alpha\ $ P t) =>$\ $?!
\onslide<3>
\lstinline![a t] refl a t --> P: hterm (a $\ \mapsto\ $o) =>$\ $h: $\varepsilon\ $($\alpha\ $ P t) =>$\ $h.!
\end{overprint}
\end{block}

\begin{block}{Remember:}
\begin{lstlisting}
[a x y] $\varepsilon$ ($\alpha\ \dot{=}$ x y) -->
  P: hterm (a $\mapsto$ o) -> $\ \varepsilon$ ($\alpha$ P x) -> $\ \varepsilon$ ($\alpha$ P y).
\end{lstlisting}
\end{block}

\end{frame}


\begin{frame}[fragile]
\frametitle{Inference rules}

\begin{itemize}
\item Every inference rule can be encoded that way
\item In fact, those rules are \alert{constant definitions}
\item Need axioms:
  \begin{itemize}
  \item classical logic
  \item axiom of choice
  \item extensionality:
  \end{itemize}
\end{itemize}

\begin{lstlisting}
f g: hterm (a $\mapsto$ b) ->
  (x: hterm a -> $\varepsilon$ ($\alpha\ \dot{=}$ ($\alpha$ f x) ($\alpha$ g x))) ->
  $\varepsilon$ ($\alpha\ \dot{=}$ f g).
\end{lstlisting}

\end{frame}


%%% Local Variables: 
%%% mode: latex
%%% TeX-master: "talk"
%%% End: 
